theories/exercises/subseg_buffer_call_ie.v
@@ -669,87 +669,24 @@ Hlink& Hentry_malloc& Hentry_assert& Hna& #Hw0& #Hadv)".
     iDestruct (region_integers_alloc' with "Hmem'") as ">#Hinterp_buffer".
     { by apply Forall_replicate. }
 
-    (* Apply the continuation *)
-
-    destruct ( decide (is_ie_cap wadv = true ) ) as [Hadv|Hadv].
-    { (* JMP TO IE-CAP ADV WITH  *)
-      iClear "Cont"; clear Cont cont0.
-      admit.
+    (* Prepare common hypotheses *)
+    assert (isCorrectPC (WCap pc_p pc_b pc_e a_end_call)).
+    { apply isCorrectPC_ExecPCPerm_InBounds ; auto.
+      assert (Hcont_clear' := Hcont_clear).
+      eapply (contiguous_between_incr_addr _ 1%nat _ f0 _)
+        in Hcont_clear'.
+      repeat (
+          match goal with
+          | h: contiguous_between _ _ _ |- _ =>
+              apply contiguous_between_bounds in h
+          end).
+      split ; auto...
+      by simplify_map_eq.
     }
 
-
-    { (* JMP TO NORMAL ADV *)
-      apply not_true_is_false in Hadv.
-      subst rmap2.
-      iExtract "Hrmap" r_t30 as "Hr30".
-      (* TODO temporarily articially bring the a_end_call *)
-      (* if I have
-         (call call_addrs ....)
-         and
-         (a_call + length call_addrs)%a = Some a_restore
-         and
-         (a_end_call + 1)%a = Some a_restore
-
-         THEN
-         (call call_addrs ....) minus the [Jmp]
-         and a_end_call -> Jmp
-
-        and the other way around
-       *)
-      rewrite /call.
-      iAssert (a_end_call ↦ₐ encodeInstrW (Jmp r_t30))%I as
-        "Hi".
-      {
-        admit.
-      }
-
-      (* Jmp adv *)
-      wp_instr.
-      iApply (wp_jmp_success with "[$HPC $Hr30 $Hi]")
-      ; [apply decode_encode_instrW_inv| |auto|..]
-      ; auto.
-      { apply isCorrectPC_ExecPCPerm_InBounds ; auto.
-        assert (Hcont_clear' := Hcont_clear).
-        eapply (contiguous_between_incr_addr _ 1%nat _ f0 _)
-          in Hcont_clear'.
-        repeat (
-            match goal with
-            | h: contiguous_between _ _ _ |- _ =>
-                apply contiguous_between_bounds in h
-            end).
-        split ; auto...
-        by simplify_map_eq.
-      }
-      iNext ; iIntros "(HPC & _ & Hr30)".
-      iInsert "Hrmap" r_t30.
-      set rmap2 := (<[r_t30:=wadv]> ( <[ r_t7 := _ ]> _)).
-      iClear "Hi".
-      wp_pure.
-
-      iSpecialize ("Cont" $! rmap2).
-      iApply "Cont" ; auto ; iFrame.
-      { iPureIntro.
-        rewrite !dom_insert_L create_gmap_default_dom list_to_set_map_to_list.
-        rewrite !dom_delete_L !dom_insert_L !dom_delete_L Hdom.
-        rewrite !singleton_union_difference_L.
-        set_solver+. }
-
-      (* -- It remains to prove that all the registers are safe to share -- *)
-      iApply big_sepM_sep. iFrame.
-      iApply big_sepM_insert_2 ; first iFrame "#". (* interp w7 *)
-      iApply big_sepM_insert_2 ; first iFrame "#". (* interp wadv *)
-      iApply big_sepM_insert_2 ; cycle 1. (* interp all \ r31 *)
-
-      (* The remaining registers contains WInt*)
-      { iApply big_sepM_intro. iIntros "!>" (r ?).
-        (set rmap' := delete r_t7 _ ).
-        destruct ((create_gmap_default (map_to_list rmap').*1 (WInt 0%Z : Word)) !! r) eqn:Hsome.
-        apply create_gmap_default_lookup_is_Some in Hsome as [Hsome ->]. rewrite !fixpoint_interp1_eq.
-        iIntros (?). simplify_eq. done. iIntros (?). done. }
-
-
-
-    (* The activation code is safe to share - ie. safe to execute *)
+    iAssert (interp (WCap RWX (b_mem ^+ (secret_off + 1))%a e_mem (b_mem ^+ secret_off)%a))%I as
+      "#Hbuffer_valid"; first iFrame "#"; iClear "Hbuffer_valid".
+    iAssert (interp (WCap IE b_act e_act b_act))%I as "Hact_valid".
     { cbn beta. rewrite !fixpoint_interp1_eq.
       iIntros (r).
       iExists (cap_eq pc_p pc_b pc_e a_restore), (cap_eq RWX b_local e_locals e_locals).
@@ -762,6 +699,7 @@ Hlink& Hentry_malloc& Hentry_assert& Hna& #Hw0& #Hadv)".
       iIntros "[%Hw1 %Hw2]" ; simplify_eq.
       (* need to consider 2 cases: w2 is context, or it is integer *)
 
+      (* TODO factor out the proof *)
       destruct Hw2 as [ -> | Hw2].
       { (* case P2 w2 *)
 
@@ -769,7 +707,7 @@ Hlink& Hentry_malloc& Hentry_assert& Hna& #Hw0& #Hadv)".
         iHide "Hinterp_buffer" as Hinterp_buffer.
         iHide "Hrmap_safe" as Hrmap_safe.
         rewrite /interp_conf /registers_mapsto.
-        apply regmap_full_dom in H as H'.
+        apply regmap_full_dom in H1 as H'.
 
 
         (* get all the registers we need for the remaining code *)
@@ -827,8 +765,7 @@ Hlink& Hentry_malloc& Hentry_assert& Hna& #Hw0& #Hadv)".
                  with "[- $HPC $Hr2 $Hr4 $Hr5 $Hlocal $Ha_secret $Hidc $Hprepa]")
         ; auto.
         { Unshelve. 2: exact prepa_addrs. cbn.
-          replace (a_prepa ^+ 4%nat)%a with a_assert by solve_addr.
-          done.
+          replace (a_prepa ^+ 4%nat)%a with a_assert by solve_addr;done.
         }
         cbn.
         split ; try solve_addr.
@@ -919,7 +856,7 @@ Hlink& Hentry_malloc& Hentry_assert& Hna& #Hw0& #Hadv)".
         iHide "Hinterp_buffer" as Hinterp_buffer.
         iHide "Hrmap_safe" as Hrmap_safe.
         rewrite /interp_conf /registers_mapsto.
-        apply regmap_full_dom in H as H'.
+        apply regmap_full_dom in H1 as H'.
 
 
         (* get all the registers we need for the remaining code *)
@@ -950,27 +887,158 @@ Hlink& Hentry_malloc& Hentry_assert& Hna& #Hw0& #Hadv)".
         iIntros (v) "% %"; simplify_eq.
       }
     }
-  Admitted.
+
+    (* Apply the continuation *)
+    destruct ( decide (is_ie_cap wadv = true ) ) as [Hadv|Hadv].
+    { (* JMP TO IE-CAP ADV WITH  *)
+      iClear "Cont"; clear Cont cont0.
+
+      destruct_word wadv ; [| destruct c | |] ; cbn in Hadv ; try congruence ; clear Hadv.
+      subst rmap2 Hinterp_adv.
+      (* prepare ressources for the jmp *)
+      iDestruct (call_main_end with "Hcall") as (call_addrs') "[-> [Hi Hcall]]" ; eauto.
+      iExtract "Hrmap" r_t30 as "Hr30".
+      assert (is_Some (rmap !! idc)) as [widc Hwidc].
+      {  clear -Hdom. apply elem_of_dom; set_solver. }
+      iDestruct ((big_sepM_delete _ _ idc (WInt 0)) with "Hrmap") as "[Hidc Hrmap]".
+      { simplify_map_eq.
+        apply create_gmap_default_lookup.
+        apply map_to_list_fst.
+        exists widc.
+        apply elem_of_map_to_list.
+        by simplify_map_eq.
+      }
+      iAssert (interp (WCap IE f f1 f2)) as "#Hadv'"; first iFrame "#".
+
+      rewrite {1}fixpoint_interp1_eq //=.
+      destruct (decide (withinBounds f f1 f2 ∧ withinBounds f f1 (f2 ^+ 1)%a))
+        as [ Hbounds | Hbounds] ; cycle 1.
+      { (* ill-formed IE, the jump fails *)
+        wp_instr.
+        iApply (wp_jmp_fail_IE with "[$HPC $Hr30 $Hidc $Hi]")
+        ; try solve_pure.
+        iNext ; iIntros "(HPC & Hr30 & _ & >Hi)".
+        wp_pure; wp_end. by iIntros "%".
+      }
+      wp_instr.
+      set (Hbounds' := Hbounds).
+      destruct Hbounds' as [Hwb Hwb'].
+      iDestruct ("Hadv" $! Hbounds)
+        as (P1 P2) "(%Hpers1 & %Hpers2 & Hinv_f1 & Hinv_f2 & Hcont)".
+
+      assert (Hf2: f2 <> (f2 ^+ 1)%a)
+        by (apply Is_true_true_1, withinBounds_true_iff in Hwb; solve_addr).
+      iInv (logN.@f2) as (w1) "[>Hf2 #HP1]" "Hcls1".
+      iInv (logN.@(f2 ^+1)%a) as (w2) "[>Hf2' #HP2]" "Hcls2".
+
+      iApply (wp_jmp_success_IE with "[$HPC $Hr30 $Hidc $Hi $Hf2 $Hf2']")
+      ; try solve_pure.
+      iNext; iIntros "(HPC& Hr30 & Hidc& Hi& Hf1& Hf2) //=".
+      iMod ("Hcls2" with "[Hf2 HP2]") as "_"; [iNext ; iExists _ ; iFrame "∗ #"| iModIntro].
+      iMod ("Hcls1" with "[Hf1 HP1]") as "_"; [iNext ; iExists _ ; iFrame "∗ #"| iModIntro].
+      iApply wp_pure_step_later; auto.
+      iNext ; iIntros "_".
+
+      iInsert "Hrmap" r_t30.
+      iDestruct (big_sepM_insert with "[Hrmap Hidc]") as "Hrmap" ; try iFrame "Hrmap Hidc".
+      { by simplify_map_eq. }
+      iDestruct (big_sepM_insert with "[Hrmap HPC]") as "Hrmap" ; try iFrame "Hrmap HPC".
+      { simplify_map_eq.
+        apply create_gmap_default_lookup_None.
+        clear -Hdom.
+        intro HPC.
+        apply map_to_list_fst in HPC.
+        destruct HPC as [wpc HPC].
+        apply elem_of_map_to_list in HPC.
+        simplify_map_eq.
+        assert (is_Some (rmap !! PC)) as Hcontra by (eexists ; eauto).
+        apply elem_of_dom in Hcontra.
+        set_solver.
+      }
+      set rmap2 := (<[PC:=w1]> ( <[idc:=w2]>  (  <[r_t30:=WCap IE f f1 f2]> _  ))).
+
+      iApply ("Hcont" $! w1 w2 rmap2); iFrame "#".
+      iSplit; cycle 1.
+      { rewrite insert_insert.
+        rewrite (insert_commute _ idc PC); [|auto].
+        rewrite insert_insert.
+        iFrame.
+      }
+      iSplit.
+      { rewrite /full_map.
+        iIntros (r) ; iPureIntro.
+        subst rmap2.
+        apply elem_of_dom.
+        rewrite !dom_insert_L !dom_delete_L !dom_insert_L create_gmap_default_dom list_to_set_map_to_list.
+        rewrite !dom_delete_L !dom_insert_L !dom_delete_L Hdom.
+        rewrite !singleton_union_difference_L.
+        set_solver.
+      }
+      {
+        iIntros (r w Hr Hr' Hregs).
+        iClear "Hadv".
+        subst rmap2.
+        do 2 (rewrite lookup_insert_ne in Hregs ; [|auto]).
+        destruct (decide (r = r_t30)); subst.
+        { rewrite lookup_insert in Hregs; simplify_eq ; iFrame "#". }
+        rewrite lookup_insert_ne in Hregs ; [|auto].
+        rewrite lookup_delete_ne in Hregs ; [|auto].
+        destruct (decide (r = r_t7)); subst.
+        { rewrite lookup_insert in Hregs; simplify_eq ; iFrame "#". }
+        rewrite lookup_insert_ne in Hregs ; [|auto].
+        destruct (decide (r = r_t31)); subst.
+        { rewrite lookup_insert in Hregs; simplify_eq ; iFrame "#". }
+        rewrite lookup_insert_ne in Hregs ; [|auto].
+        apply create_gmap_default_lookup_is_Some in Hregs.
+        destruct Hregs as [_ ->]. rewrite !fixpoint_interp1_eq; auto.
+      }
+    }
 
 
 
+    (* --------------------------------------------------------------------- *)
+
+    { (* JMP TO NORMAL ADV *)
+      apply not_true_is_false in Hadv.
+      subst rmap2.
+      iExtract "Hrmap" r_t30 as "Hr30".
 
 
+      iDestruct (call_main_end with "Hcall") as (call_addrs') "[-> [Hi Hcall]]" ; eauto.
+
+      (* Jmp adv *)
+      wp_instr.
+      iApply (wp_jmp_success with "[$HPC $Hr30 $Hi]")
+      ; [apply decode_encode_instrW_inv| |auto|..]
+      ; auto.
+      iNext ; iIntros "(HPC & Hi & Hr30)".
+      iInsert "Hrmap" r_t30.
+      set rmap2 := (<[r_t30:=wadv]> ( <[ r_t7 := _ ]> _)).
+      iClear "Hi".
+      wp_pure.
+
+      iSpecialize ("Cont" $! rmap2).
+      iApply "Cont" ; auto ; iFrame.
+      { iPureIntro.
+        rewrite !dom_insert_L create_gmap_default_dom list_to_set_map_to_list.
+        rewrite !dom_delete_L !dom_insert_L !dom_delete_L Hdom.
+        rewrite !singleton_union_difference_L.
+        set_solver+. }
 
 
+      (* -- It remains to prove that all the registers are safe to share -- *)
+      iApply big_sepM_sep. iFrame.
+      iApply big_sepM_insert_2 ; first iFrame "#". (* interp w7 *)
+      iApply big_sepM_insert_2 ; first iFrame "#". (* interp wadv *)
+      iApply big_sepM_insert_2 ; first iFrame "#". (* interp wadv *)
 
-
-
-
-
-
-
-
-
-
-
-
-
+      (* The remaining registers contains WInt*)
+      { iApply big_sepM_intro. iIntros "!>" (r ?).
+        (set rmap' := delete r_t7 _ ).
+        destruct ((create_gmap_default (map_to_list rmap').*1 (WInt 0%Z : Word)) !! r) eqn:Hsome.
+        apply create_gmap_default_lookup_is_Some in Hsome as [Hsome ->]. rewrite !fixpoint_interp1_eq.
+        iIntros (?). simplify_eq. done. iIntros (?). done. }
+    }
   Qed.
 
   (* The post-condition actually does not matter *)
